Updated notations for smaller spec memory footprint.

src/QueryStructure/Specification/Operations/Insert.v
@@ -31,73 +31,73 @@ Proof.
   firstorder.
 Qed.
 
-Locate GetRelation.
-
 Definition QSInsertSpec
-           (qs : QueryStructureHint)
+           {qs_schema}
+           (qs : QueryStructure qs_schema)
            (Ridx : Fin.t _)
-           (tup : @IndexedRawTuple (GetNRelSchemaHeading (qschemaSchemas qsSchemaHint') Ridx))
-           (qs' : QueryStructure qsSchemaHint')
+           (tup : @IndexedRawTuple (GetNRelSchemaHeading (qschemaSchemas qs_schema) Ridx))
+           (qs' : QueryStructure qs_schema)
 : Prop :=
   (* All of the relations with a different index are untouched
      by insert. *)
   (forall Ridx',
      Ridx <> Ridx' ->
-     GetRelation qsHint Ridx' = GetRelation qs' Ridx') /\
+     GetRelation qs Ridx' = GetRelation qs' Ridx') /\
   (* If [tup] is consistent with the schema constraints, *)
   (SatisfiesAttributeConstraints Ridx (indexedElement tup))
   -> (forall tup',
-        GetRelation qsHint Ridx tup'
+        GetRelation qs Ridx tup'
         -> SatisfiesTupleConstraints Ridx (indexedElement tup) (indexedElement tup'))
   -> (forall tup',
-        GetRelation qsHint Ridx tup'
+        GetRelation qs Ridx tup'
         -> SatisfiesTupleConstraints Ridx (indexedElement tup') (indexedElement tup))
   (* and [tup] is consistent with the other tables per the cross-relation
      constraints, *)
   -> (forall Ridx', SatisfiesCrossRelationConstraints Ridx Ridx' (indexedElement tup)
-                                                      ((GetRelation qsHint Ridx')))
+                                                      ((GetRelation qs Ridx')))
   (* and each tuple in the other tables is consistent with the
      table produced by inserting [tup] into the relation indexed by [Ridx], *)
   -> (forall Ridx',
         Ridx' <> Ridx ->
         forall tup',
-        (GetRelation qsHint Ridx') tup'
+        (GetRelation qs Ridx') tup'
         -> SatisfiesCrossRelationConstraints
              Ridx' Ridx (indexedElement tup')
-             (EnsembleInsert tup ((GetRelation qsHint Ridx))))
+             (EnsembleInsert tup ((GetRelation qs Ridx))))
   (* [tup] is included in the relation indexed by [Ridx] after insert.
    The behavior of insertion is unspecified otherwise. *)
   -> (forall t, GetRelation qs' Ridx t <->
-                (EnsembleInsert tup (GetRelation qsHint Ridx) t)).
+                (EnsembleInsert tup (GetRelation qs Ridx) t)).
 
-Definition freshIdx (qs : QueryStructureHint) Ridx (n : nat) :=
+Definition freshIdx {qs_schema} (qs : QueryStructure qs_schema) Ridx (n : nat) :=
   forall tup,
-    GetRelation qsHint Ridx tup ->
+    GetRelation qs Ridx tup ->
     RawTupleIndex tup <> n.
 
 Definition SuccessfulInsertSpec
-           (qs : QueryStructureHint)
+           {qs_schema}
+           (qs : QueryStructure qs_schema)
            (Ridx : _)
-           (qs' : QueryStructure qsSchemaHint')
-           (tup : @IndexedRawTuple (GetNRelSchemaHeading (qschemaSchemas qsSchemaHint') Ridx))
+           (qs' : QueryStructure qs_schema)
+           (tup : @IndexedRawTuple (GetNRelSchemaHeading (qschemaSchemas qs_schema) Ridx))
            (result : bool) : Prop :=
   decides result (forall t,
                GetRelation qs' Ridx t <->
                (EnsembleInsert tup
-                               (GetRelation qsHint Ridx) t)).
+                               (GetRelation qs Ridx) t)).
 
-Definition QSInsert (qs : QueryStructureHint) Ridx tup :=
-  (idx <- Pick (freshIdx _ Ridx);
-   qs' <- Pick (QSInsertSpec _ Ridx {| elementIndex := idx;
+Definition QSInsert {qs_schema} (qs : QueryStructure qs_schema) Ridx tup :=
+  (idx <- Pick (freshIdx qs Ridx);
+   qs' <- Pick (QSInsertSpec qs Ridx {| elementIndex := idx;
                                       indexedElement := tup |});
-   b <- Pick (SuccessfulInsertSpec _ Ridx qs'
+   b <- Pick (SuccessfulInsertSpec qs Ridx qs'
                                    {| elementIndex := idx;
                                       indexedElement := tup |});
    ret (qs', b))%comp.
 
 Opaque QSInsert.
 
-Notation "'Insert' b 'into' Ridx " :=
-  (QSInsert _
-            (ibound (indexb (@Build_BoundedIndex _ _ (QSschemaNames qsSchemaHint) Ridx%string _))) b)
-    (at level 80) : QuerySpec_scope.
+Notation "'Insert' b 'into' r '!' Ridx " :=
+  (QSInsert r
+            (ibound (indexb (@Build_BoundedIndex _ _ (QSschemaNames _) Ridx%string _))) b)
+    (r at level 0, at level 0) : QuerySpec_scope.
