src/Examples/QueryStructure/Bookstore.v
@@ -69,39 +69,41 @@ Definition BookStoreSig : ADTSig :=
 (* Now we write what the methods should actually do. *)
 
 Definition BookStoreSpec : ADT BookStoreSig :=
-  Eval simpl in 
-  QueryADTRep BookStoreSchema {
+  Eval simpl in
+    QueryADTRep BookStoreSchema {
     Def Constructor "Init" (_ : unit) : rep := empty,
 
-    update "PlaceOrder" ( o : Order ) : bool :=
-        Insert o into sORDERS,
+    update "PlaceOrder" ( r : rep , o : Order ) : bool :=
+        Insert o into r!sORDERS,
 
-    update "DeleteOrder" ( oid : nat ) : list Order :=
-      Delete o from sORDERS where o!sISBN = oid,
+    update "DeleteOrder" (r : rep, oid : nat ) : list Order :=
+       Delete o from r!sORDERS where True,
 
-    update "AddBook" ( b : Book ) : bool :=
-        Insert b into sBOOKS ,
+    update "AddBook" (r : rep, b : Book ) : bool :=
+        Insert b into r!sBOOKS ,
 
-     update "DeleteBook" ( id : nat ) : list Book :=
-        Delete book from sBOOKS where book!sISBN = id ,
+     update "DeleteBook" ( r : rep, id : nat ) : list Book :=
+        Delete book from r!sBOOKS where book!sISBN = id,
 
-    query "GetTitles" ( author : string ) : list string :=
-      For (b in sBOOKS)
+    query "GetTitles" (r : rep, author : string ) : list string :=
+      For (b in r ! sBOOKS)
       Where (author = b!sAUTHOR)
-      Return (b!sTITLE) ,
+      Return (b!sTITLE),
 
-    query "NumOrders" ( author : string ) : nat :=
-      Count (For (o in sORDERS) (b in sBOOKS)
+    query "NumOrders" (r : rep, author : string ) : nat :=
+      Count (For (o in r!sORDERS) (b in r!sBOOKS)
                  Where (author = b!sAUTHOR)
-                 Where (b!sISBN = o!sISBN)
+                 Where (o!sISBN = b!sISBN)
                  Return ())
 }.
 
 Theorem SharpenedBookStore :
   MostlySharpened BookStoreSpec.
 Proof.
+
   Time start honing QueryStructure.
-  (* 552 MB. *)
+
+  (* 552 MB vs 624MB. *)
   partial_master_plan EqIndexTactics.
 
   FullySharpenQueryStructure BookStoreSchema Index.
